---
title: 1. Natural Numbers
# description: Short summary of the post
date: 2025-01-01 20:49
categories: [Mathematics, Analysis]
tags: [analysis, natural-number, peano-axiom]     # TAG names should always be lowercase
math: true
pin: false
---

## 1.1 The Peano axioms

### Definition 1.1.1 (informal)

A natural number is any element of the set

$$
\begin{align*}
    \mathbf{N} := \{ 0, \ 1, \ 2, \ 3, \ 4, \dots \}
\end{align*}
$$

which is the set of all numbers created by starting with $$ 0 $$ and then counting forward indefinitely.

### Axiom 1.1

$$ 0 $$ is a natural number.

### Axiom 1.2

If $$ n $$ is a natural number, then $$ n++ $$ is also a natural number.

### Definition 1.1.2

We define $$ 1 $$ to be the number $$ 0++ $$, $$ 2 $$ to be the number $$ (0++)++ $$, $$ 3 $$ to be the number $$ ((0++)++)++ $$, etc.

### Proposition 1.1.3

$$ 3 $$ is a natural number.

**Proof**  
By Axiom 1.1, $$ 0 $$ is a natural number.
By Axiom 1.2, $$ 0++ = 1 $$ is a natural number.
By Axiom 1.2 again, $$ 1++ = 2 $$ is a natural number.
By Axiom 1.2 again, $$ 2++ = 3 $$ is a natural number. $$ \blacksquare $$

### Axiom 1.3

$$ 0 $$ is not the successor of any natural number; i.e., we have $$ n++ \neq 0 $$ for every natural number $$ n $$.

### Proposition 1.1.4

$$ 4 $$ is not equal to $$ 0 $$.

**Proof**  
By definition, $$ 4 = 3++ $$.
By Axioms 1.1 and 1.2, $$ 3 $$ is a natural number.
Thus by Axiom 1.3, $$ 3++ \neq 0 $$, i.e., $$ 4 \neq 0 $$. $$ \blacksquare $$

### Axiom 1.4

Different natural numbers must have different successors; i.e., if $$ n $$, $$ m $$ are natural numbers and $$ n \neq m $$, then $$ n++ \neq m++ $$.
Equivalently, if $$ n++ = m++ $$ then we must have $$ n = m $$.

### Proposition 1.1.5

$$ 6 $$ is not equal to $$ 2 $$.

**Proof**  
Suppose for sake of contradiction that $$ 6 = 2 $$.
Then $$ 5++ = 1++ $$, so by Axiom 1.4 we have $$ 5 = 1 $$, so that $$ 4++ = 0++ $$.
By Axiom 1.4 again we then have $$ 4 = 0 $$, which contradicts our previous proposition. $$ \blacksquare $$

### Axiom 1.5 (principle of mathematical induction)

Let $$ P(n) $$ be any property pertaining to a natural number $$ n $$.
Suppose that $$ P(0) $$ is true, and suppose that whenever $$ P(n) $$ is true, $$ P(n++) $$ is also true.
Then $$ P(n) $$ is true for every natural number $$ n $$.

Axioms 1.1â€“1.5 are known as the Peano axioms for the natural numbers.

### Proposition 1.1.6 (recursive definitions)

Suppose for each natural number $$ n $$, we have some function $$ f_n : \mathbf{N} \rightarrow \mathbf{N} $$ from the natural numbers to the natural numbers.
Let $$ c $$ be a natural number.
Then we can assign a unique natural number $$ a_n $$ to each natural number $$ n $$, such that $$ a_0 = c $$ and $$ a_{n++} = f_n(a_n) $$ for each natural number $$ n $$.

**Proof (informal)**  
We use induction.
We first observe that this procedure gives a single value to $$ a_0 $$, namely $$ c $$.
(None of the other definitions $$ a_{n++} := f_n(a_n) $$ will redefine the value of $$ a_0 $$, because of Axiom 1.3.)
Now suppose inductively that the procedure gives a single value to $$ a_n $$.
Then it gives a single value to $$ a_{n++} $$, namely $$ a_{n++} := f_n(a_n) $$.
(None of the other definitions $$ a_{m++} := f_m(a_m) $$ will redefine the value of $$ a_{n++ } $$, because of Axiom 1.4.)
This completes the induction, and so $$ a_n $$ is defined for each natural number $$ n $$, with a single value assigned to each $$ a_n $$. $$ \blacksquare $$

## 1.2 Addition

### Definition 1.2.1 (addition of natural numbers)

Let $$ m $$ be a natural number.
To add zero to $$ m $$, we define $$ 0 + m := m $$.
Now suppose inductively that we have defined how to add $$ n $$ to $$ m $$.
Then we can add $$ n++ $$ to $$ m $$ by defining $$ (n++) + m := (n + m)++ $$.

### Lemma 1.2.2

For any natural number $$ n $$, $$ n + 0 = n $$.

**Proof**  
We use induction.
The base case $$ 0 + 0 = 0 $$ follows since we know that $$ 0 + m = m $$ for every natural number $$ m $$, and $$ 0 $$ is a natural number.
Now suppose inductively that $$ n + 0 = n $$.
By definition of addition, $$ (n++) + 0 $$ is equal to $$ (n + 0)++ $$, which is equal to $$ n++ $$ since $$ n + 0 = n $$.
This closes the induction. $$ \blacksquare $$

### Lemma 1.2.3

For any natural numbers $$ n $$ and $$ m $$, $$ n + (m++) = (n + m)++ $$.

**Proof**  
We induct on $$ n $$ (keeping $$ m $$ fixed).
We first consider the base case $$ n = 0 $$.
In this case we have to prove $$ 0 + (m++) = (0 + m)++ $$.
But by definition of addition, $$ 0 + (m++) = m++ $$ and $$ 0 + m = m $$, so both sides are equal to $$ m++ $$ and are thus equal to each other.
Now we assume inductively that $$ n + (m++) = (n + m)++ $$; we now have to show that $$ (n++) + (m++) = ((n++) + m)++ $$.
The left-hand side is $$ (n + (m++))++ $$ by definition of addition, which is equal to $$ ((n + m)++)++ $$ by the inductive hypothesis.
Similarly, we have $$ (n++) + m = (n + m)++ $$ by the definition of addition, and so the right-hand side is also equal to $$ ((n + m)++)++ $$.
Thus both sides are equal to each other, and we have closed the induction. $$ \blacksquare $$

### Proposition 1.2.4 (addition is commutative)

For any natural numbers $$ n $$ and $$ m $$, $$ n + m = m + n $$.

**Proof**  
We shall use induction on $$ n $$ (keeping $$ m $$ fixed).
First we do the base case $$ n = 0 $$, i.e., we show $$ 0 + m = m + 0 $$.
By the definition of addition, $$ 0 + m = m $$, while by Lemma 1.2.2, $$ m + 0 = m $$.
Thus the base case is done.
Now suppose inductively that $$ n + m = m + n $$.
By the definition of addition, $$ (n++) + m = (n + m)++ $$.
By Lemma 1.2.3, $$ m + (n++) = (m + n)++ $$, but this is equal to $$ (n + m)++ $$ by the inductive hypothesis $$ n + m = m + n $$.
Thus $$ (n++) + m = m + (n++) $$ and we have closed the induction. $$ \blacksquare $$

### Proposition 1.2.5 (addition is associative)

For any natural numbers $$ a $$, $$ b $$, $$ c $$, we have $$ (a + b) + c = a + (b + c) $$.

### Proposition 1.2.6 (cancellation law)

Let $$ a $$, $$ b $$, $$ c $$ be natural numbers such that $$ a + b = a + c $$.
Then we have $$ b = c $$.

**Proof**  
We prove this by induction on $$ a $$.
First consider the base case $$ a = 0 $$.
Then we have $$ 0 + b = 0 + c $$, which by definition of addition implies that $$ b = c $$ as desired.
Now suppose inductively that we have the cancellation law for $$ a $$ (so that $$ a + b = a + c $$ implies $$ b = c $$).
We now have to assume that $$ (a++) + b = (a++) + c $$ and show that $$ b = c $$.
By the definition of addition, $$ (a++) + b = (a + b)++ $$ and $$ (a++) + c = (a + c)++ $$ and so we have $$ (a + b)++ = (a + c)++ $$.
By Axiom 1.4, we have $$ a + b = a + c $$, thus we have $$ b = c $$. $$ \blacksquare $$

### Definition 1.2.7 (positive natural numbers)

A natural number $$ n $$ is said to be positive iff it is not equal to $$ 0 $$.

### Proposition 1.2.8

If $$ a $$ is a positive natural number, and $$ b $$ is a natural number, then $$ a + b $$ is positive.

**Proof**  
We use induction on $$ b $$.
If $$ b = 0 $$, then $$ a + b = a + 0 = a $$, which is positive.
Now suppose inductively that $$ a + b $$ is positive.
Then $$ a + (b++) = (a + b)++ $$, which cannot be zero by Axiom 1.3, and is hence positive. $$ \blacksquare $$

### Corollary 1.2.9

If $$ a $$ and $$ b $$ are natural numbers such that $$ a + b = 0 $$, then $$ a = 0 $$ and $$ b = 0 $$.

**Proof**  
Suppose that $$ a \neq 0 $$ and $$ b \neq 0 $$.
If $$ a \neq 0 $$ then $$ a $$ is positive, and hence $$ a + b = 0 $$ is positive by Proposition 1.2.8, a contradiction.
Similarly if $$ b \neq 0 $$ then $$ b $$ is positive, and again $$ a + b = 0 $$ is positive by Proposition 1.2.8, a contradiction.
Thus $$ a $$ and $$ b $$ must both be zero. $$ \blacksquare $$

### Lemma 1.2.10

Let $$ a $$ be a positive number.
Then there exists exactly one natural number $$ b $$ such that $$ b++ = a $$.

### Definition 1.2.11 (ordering of natural numbers)

Let $$ n $$ and $$ m $$ be natural numbers.
We say that $$ n $$ is greater than or equal to $$ m $$, and write $$ n \ge m $$ or $$ m \le n $$, iff we have $$ n = m + a $$ for some natural number $$ a $$.
We say that $$ n $$ is strictly greater than $$ m $$, and write $$ n > m $$ or $$ m < n $$, iff $$ n \ge m $$ and $$ n \neq m $$.

### Proposition 1.2.12 (basic properties of order for natural numbers)

Let $$ a $$, $$ b $$, $$ c $$ be natural numbers.
Then  
(a) (order is reflexive) $$ a \ge a $$.  
(b) (order is transitive) If $$ a \ge b $$ and $$ b \ge c $$, then $$ a \ge c $$.  
(c) (order is antisymmetric) If $$ a \ge b $$ and $$ b \ge a $$, then $$ a = b $$.  
(d) (addition preserves order) $$ a \ge b $$ if and only if $$ a + c \ge b + c $$.  
(e) $$ a < b $$ if and only if $$ a++ \le b $$.  
(f) $$ a < b $$ if and only if $$ b = a + d $$ for some positive number $$ d $$.

### Proposition 1.2.13 (trichotomy of order for natural numbers)

Let $$ a $$ and $$ b $$ be natural numbers.
Then exactly one of the following statements is true: $$ a < b $$, $$ a = b $$, or $$ a > b $$.

### Proposition 1.2.14 (strong principle of induction)

Let $$ m_0 $$ be a natural number, and let $$ P(m) $$ be a property pertaining to an arbitrary natural number $$ m $$.
Suppose that for each $$ m \ge m_0 $$, we have the following implication: if $$ P'(m) $$ is true for all natural numbers $$ m_0 \le m' < m $$, then $$ P(m) $$ is also true.
(In particular, this means that $$ P(m_0) $$ is true, since in this case the hypothesis is vacuous.)
Then we can conclude that $$ P(m) $$ is true for all natural numbers $$ m \ge m_0 $$.

## 1.3 Multiplication

### Definition 1.3.1 (multiplication of natural numbers)

Let $$ m $$ be a natural number.
To multiply zero to $$ m $$, we define $$ 0 \times m := 0 $$.
Now suppose inductively that we have defined how to multiply $$ n $$ to $$ m $$.
Then we can multiply $$ n++ $$ to $$ m $$ by defining $$ (n++) \times m := (n \times m) + m $$.

### Lemma 1.3.2 (multiplication is commutative)

Let $$ n $$, $$ m $$ be natural numbers.
Then $$ n \times m = m \times n $$.

We will now abbreviate $$ n \times m $$ as $$ nm $$.

### Lemma 1.3.3 (positive natural numbers have no zero divisors)

Let $$ n $$, $$ m $$ be natural numbers.
Then $$ n \times m = 0 $$ if and only if at least one of $$ n $$, $$ m $$ is equal to zero.
In particular, if $$ n $$ and $$ m $$ are both positive, then $$ nm $$ is also positive.

### Proposition 1.3.4 (distributive law)

For any natural numbers $$ a $$, $$ b $$, $$ c $$, we have $$ a(b + c) = ab + ac $$ and $$ (b + c)a = ba + ca $$.

**Proof**  
Since multiplication is commutative we only need to show the first identity $$ a(b + c) = ab + ac $$.
We keep $$ a $$ and $$ b $$ fixed, and use induction on $$ c $$.
Let $$ c = 0 $$, i.e., $$ a(b + 0) = ab + a0 $$.
The left-hand side is $$ ab $$, while the right-hand side is $$ ab + 0 = ab $$.
Now let us suppose inductively that $$ a(b + c) = ab + ac $$, and let us prove that $$ a(b + (c++)) = ab + a(c++) $$.
The left-hand side is $$ a((b + c)++) = a(b + c) + a $$, while the right-hand side is $$ ab + ac + a = a(b + c) + a $$ by the induction hypothesis, and so we can close the induction. $$ \blacksquare $$

### Proposition 1.3.5 (multiplication is associative)

For any natural numbers $$ a $$, $$ b $$, $$ c $$, we have $$ (a \times b) \times c = a \times (b \times c) $$.

### Proposition 1.3.6 (multiplication preserves order)

If $$ a $$, $$ b $$ are natural numbers such that $$ a < b $$, and $$ c $$ is positive, then $$ ac < bc $$.

**Proof**  
Since $$ a < b $$, we have $$ b = a + d $$ for some positive $$ d $$.
Multiplying by $$ c $$ and using the distributive law we obtain $$ bc = ac + dc $$.
Since $$ d $$ is positive, and $$ c $$ is positive, $$ dc $$ is positive, and hence $$ ac < bc $$ as desired. $$ \blacksquare $$

### Corollary 1.3.7 (cancellation law)

Let $$ a $$, $$ b $$, $$ c $$ be natural numbers such that $$ ac = bc $$ and $$ c $$ is non-zero.
Then $$ a = b $$.

**Proof**  
By the trichotomy of order (Proposition 1.2.13), we have three cases: $$ a < b $$, $$ a = b $$, $$ a > b $$.
Suppose first that $$ a < b $$, then by Proposition 1.3.6 we have $$ ac < bc $$, a contradiction.
We can obtain a similar contradiction when $$ a > b $$.
Thus the only possibility is that $$ a = b $$. $$ \blacksquare $$

### Proposition 1.3.8 (Euclid's division lemma)

Let $$ n $$ be a natural number, and let $$ q $$ be a positive number.
Then there exist natural numbers $$ m $$, $$ r $$ such that $$ 0 \le r < q $$ and $$ n = mq + r $$.

### Definition 1.3.9 (exponentiation for natural numbers)

Let $$ m $$ be a natural number.
To raise $$ m $$ to the power $$ 0 $$, we define $$ m^0 := 1 $$; in particular, we define $$ 0^0 := 1 $$.
Now suppose recursively that $$ m^n $$ has been defined for some natural number $$ n $$, then we define $$ m^{n++} := m^n \times m $$.

---

Sources:
- [Tao, T. (2022). Analysis I (4th ed.). Hindustan Book Agency.](https://a.co/d/4m0Ex21)